\documentclass{article}
\usepackage{ifthen}
\usepackage{epsfig}
\usepackage[utf8]{inputenc}
\usepackage{newunicodechar}
  \newunicodechar{⁻}{${}^{-}$}% Superscript minus
  \newunicodechar{²}{${}^{2}$}% Superscript two
  \newunicodechar{³}{${}^{3}$}% Superscript three

\pagestyle{empty}
\begin{document}
\begin{eqnarray*} D &=& \text{the dimension of the array}\\ % N &=& \text{depth of the loop nest}\\ % V &=& \text{runtime variables}\\ % \textbf{i}\in\mathbb{R}^N &=& \text{the old index vector}\\ % \textbf{j}\in\mathbb{R}^N &=& \text{the new index vector}\\ % \textbf{x}\in\mathbb{R}^D &=& \text{the indices into the array}\\ % \textbf{M}\in\mathbb{R}^{N \times D} &=& \text{map from loop ind vars to array indices}\\ % \boldsymbol{\Phi}\in\mathbb{R}^{N \times N} &=& \text{the schedule matrix}\\ % \boldsymbol{\omega}\in\mathbb{R}^N &=& \text{the offset vector}\\ % \textbf{c}\in\mathbb{R}^{N} &=& \text{the constant offset vector}\\ % \textbf{C}\in\mathbb{R}^{N \times V} &=& \text{runtime variable coefficient matrix}\\ % \textbf{s}\in\mathbb{R}^V &=& \text{the symbolic runtime variables}\\ % \end{eqnarray*}
\pagebreak

$\boldsymbol{\Phi}$
\pagebreak

\begin{eqnarray*} \textbf{j} &=& \boldsymbol{\Phi}\textbf{i} + \boldsymbol{\omega}\\ % \textbf{i} &=& \boldsymbol{\Phi}^{-1}\left(j - \boldsymbol{\omega}\right)\\ % \textbf{x} &=& \textbf{M}'\textbf{i} + \textbf{c} + \textbf{Cs} \\ % \textbf{x} &=& \textbf{M}'\boldsymbol{\Phi}^{-1}\left(j - \boldsymbol{\omega}\right) + \textbf{c} + \textbf{Cs} \\ % \textbf{M}'_* &=& \textbf{M}'\boldsymbol{\Phi}^{-1}\\ % \textbf{x} &=& \textbf{M}'_*\left(j - \boldsymbol{\omega}\right) + \textbf{c} + \textbf{Cs} \\ % \textbf{x} &=& \textbf{M}'_*j - \textbf{M}'_*\boldsymbol{\omega} + \textbf{c} + \textbf{Cs} \\ % \textbf{c}_* &=& \textbf{c} - \textbf{M}'_*\boldsymbol{\omega} \\ % \textbf{x} &=& \textbf{M}'_*j + \textbf{c}_* + \textbf{Cs} \\ % \end{eqnarray*}
\pagebreak

$\textbf{c}_*$
\pagebreak

$\textbf{M}'_*$
\pagebreak

$\boldsymbol{\Phi} = \textbf{E}$
\pagebreak

$\textbf{AX} = \textbf{B}$
\pagebreak

$\textbf{W}$
\pagebreak

$\textbf{A}$
\pagebreak

$\textbf{D}$
\pagebreak

$\textbf{B}$
\pagebreak

$\textbf{D}^{-1}\textbf{B} = \textbf{A}^{-1}$
\pagebreak

$s$
\pagebreak

$\frac{1}{s}\textbf{B} = \textbf{A}^{-1}$
\pagebreak

\end{document}
